\section{Appendix A: Answers to inline questions}
\subsection{Question 1}
\begin{equation*}
y[n] = z[Mn]
\end{equation*}
\begin{equation*}
z[n] = \sum_{0\leq j < 4L} h[j] \cdot q[n-j]
\end{equation*}
\begin{equation*}
q[n] = \begin{cases}
x[n \text{ div } L]&\text{if } n \bmod L = 0\\
0&\text{otherwise}
\end{cases}
\end{equation*}
\begin{equation*}
y[n] = \sum_{0\leq j<4L} h[j] \cdot q[nM-j]
\end{equation*}
\begin{equation*}
y[n] = \begin{cases}
\sum_{0 \leq j < 4L} h[j] \cdot q[(nM-j) \text{ div } L]&\text{if } (nM - j) \bmod L = 0\\
\sum_{0 \leq j < 4L} h[j] \cdot 0 &\text{otherwise}
\end{cases}
\end{equation*}
The \emph{otherwise} case is always 0 so doesn't contribute to the sum.
We can continue with just:
\begin{equation*}
y[n] = \sum_{0\leq j<4L} h[j] \cdot q[(nM-j) \text{ div } L])  \phantom{xxx}\text{ if } (nM-j) \bmod L = 0
\end{equation*}
$(nM-j) \bmod L = 0$  happens at:
\begin{itemize}
\item $  j = nM \bmod L$
\item $  j = nM \bmod L + L$
\item $  j = nM \bmod L + 2L$
\item $  j = nM \bmod L + 3L$
\end{itemize}
So four times in every summation. If we let $j$ run from $0$ to $4$ (excl),
we get $h[nM \bmod L + jL]$.
\begin{equation*}
y[n] = \sum_{0\leq j<4} h[nM \bmod L + jL] \cdot q[(nM-j \cdot L) \text{ div } L]
\end{equation*}
\begin{equation*}
y[n] = \sum_{0\leq j<4} h[nM \bmod L + jL] \cdot q[(nM) \text{ div } L - j]
\end{equation*}
Which is the equation from the assignment. 

\subsection{Question 2}
\subsection{Question 3}
\section{Appendix B: Verilog source code}
This appendix includes Verilog source code for the \texttt{filter.v} file in the ISE project.

\begin{verbatim}
\end{verbatim}
